theories/examples/lse.v
@@ -11,11 +11,11 @@ Proof.
   intros l Hl Hdup.
   assert (i ∈ (map_to_list m).*1) as Hin.
   { rewrite -Hl. constructor. }
-  apply NoDup_cons_iff in Hdup as [Hnin Hdup]. 
-  apply Permutation.NoDup_Permutation;auto. 
+  apply NoDup_cons_iff in Hdup as [Hnin Hdup].
+  apply Permutation.NoDup_Permutation;auto.
   apply NoDup_map_to_list_fst. done.
   set l' := zip l (repeat x (length l)).
-  assert (l = l'.*1) as Heq;[rewrite fst_zip;auto;rewrite repeat_length;lia|]. 
+  assert (l = l'.*1) as Heq;[rewrite fst_zip;auto;rewrite repeat_length;lia|].
   intros i0. split.
   - intros Hinx%elem_of_list_In%elem_of_list_fmap.
     destruct Hinx as [ [? ?] [? Hinx] ]. simpl in *. subst a.
@@ -26,9 +26,9 @@ Proof.
     assert (i0 ∈ (map_to_list m).*1) as Hinx'.
     { apply elem_of_list_fmap. exists (i0,b). split;auto. }
     revert Hinx'. rewrite -Hl =>Hinx'. apply elem_of_cons in Hinx' as [Hcontr | Hinx'];[congruence|].
-    apply elem_of_list_In;auto. 
+    apply elem_of_list_In;auto.
   - intros Hinx%elem_of_list_In.
-    apply elem_of_list_In. revert Hnin; rewrite -elem_of_list_In => Hnin. 
+    apply elem_of_list_In. revert Hnin; rewrite -elem_of_list_In => Hnin.
     assert (i ≠ i0) as Hne;[congruence|simplify_map_eq].
     assert (i0 ∈ i :: l) as Hin'.
     { constructor. auto. }
@@ -36,7 +36,7 @@ Proof.
     apply map_to_list_fst in Hin' as [x' Hx].
     apply elem_of_map_to_list in Hx.
     apply map_to_list_fst. exists x'. apply elem_of_map_to_list.
-    rewrite lookup_delete_ne;auto. 
+    rewrite lookup_delete_ne;auto.
 Qed.
 
 Lemma big_sepM_to_create_gmap_default {Σ : gFunctors} {A B : Type} `{Countable A} (m m' : gmap A B) (φ : A -> B -> iProp Σ) (b : B) (l : list A) :
@@ -45,8 +45,8 @@ Lemma big_sepM_to_create_gmap_default {Σ : gFunctors} {A B : Type} `{Countable 
   ([∗ map] a↦_ ∈ m, φ a b) -∗ ([∗ map] a↦b' ∈ m', φ a b').
 Proof.
   iIntros (Hl Hm) "Hm".
-  iInduction l as [|a l] "IH" forall (m m' Hl Hm). 
-  - simpl in Hm. rewrite Hm. done. 
+  iInduction l as [|a l] "IH" forall (m m' Hl Hm).
+  - simpl in Hm. rewrite Hm. done.
   - assert (NoDup (a :: l)) as Hdup.
     { rewrite Hl. apply NoDup_map_to_list_fst. done. }
     assert (a ∈ (map_to_list m).*1) as Hin'.
@@ -57,17 +57,17 @@ Proof.
     iApply big_sepM_delete;[|iFrame].
     { rewrite Hm.  apply lookup_insert. }
     rewrite Hm /= delete_insert_delete.
-    iApply ("IH" $! (delete a m));[..|iFrame]. 
-    + iPureIntro. rewrite map_to_list_delete_fst;eauto. 
+    iApply ("IH" $! (delete a m));[..|iFrame].
+    + iPureIntro. rewrite map_to_list_delete_fst;eauto.
     + iPureIntro. rewrite delete_notin;auto.
-      destruct (create_gmap_default l b !! a) eqn:Hsome';auto. 
+      destruct (create_gmap_default l b !! a) eqn:Hsome';auto.
       exfalso. apply NoDup_cons_iff in Hdup as [Hnin Hdup].
       apply Hnin. apply elem_of_list_In.
       apply create_gmap_default_lookup_is_Some in Hsome' as [Hin Hsome']. subst.
-      auto. 
-Qed. 
-    
-    
+      auto.
+Qed.
+
+
 Section roe.
   Context {Σ:gFunctors} {memg:memG Σ} {regg:regG Σ}
           {nainv: logrel_na_invs Σ}
@@ -83,7 +83,7 @@ Section roe.
     malloc_instrs f_m 1%nat ++
     [move_r r_env r_t1;
     move_r r_t7 r_t1;
-    store_z r_env 1; 
+    store_z r_env 1;
     restrict_z r_t7 ro] ++
     call_instrs f_m (offset_to_cont_call [r_t7]) r1 [r_env] [r_t7] ++
     restore_locals_instrs r_t2 [r_env] ++
@@ -128,10 +128,10 @@ Section roe.
     (a_link + f_m)%a = Some a_entry →
     (a_link + f_a)%a = Some a_entry' →
     (fail_start + strings.length (assert_fail_instrs))%a = Some a_env →
-    
+
     (* footprint of the register map *)
     dom (gset RegName) rmap = all_registers_s ∖ {[PC;r_adv]} →
-    
+
     {{{ PC ↦ᵣ WCap pc_p pc_b pc_e a_first
       ∗ r_adv ↦ᵣ wadv
       ∗ ([∗ map] r_i↦w_i ∈ rmap, r_i ↦ᵣ w_i)
@@ -141,7 +141,7 @@ Section roe.
       ∗ roe roe_addrs f_m f_a r_adv
       (* untrusted code *)
       ∗ interp wadv
-      
+
       (** Resources for malloc and assert **)
       (* assume that a pointer to the linking table (where the malloc capa is) is at offset 0 of PC *)
       ∗ na_inv logrel_nais mallocN (malloc_inv b_m e_m)
@@ -153,18 +153,18 @@ Section roe.
       ∗ (inv roeN_flag (flag_a ↦ₐ WInt 0%Z))
     }}}
       Seq (Instr Executable)
-      {{{ v, RET v; True }}}. (* in this spec, we do not care about the postcondition, 
-                              only that the flag invariant holds throughout the program, 
+      {{{ v, RET v; True }}}. (* in this spec, we do not care about the postcondition,
+                              only that the flag invariant holds throughout the program,
                               and that the program does not get stuck *)
   Proof.
-    iIntros (Hvpc Hcont Hwb1 Hwb2 Ha_entry Ha_entry' Ha_env Hdom φ) 
-            "(HPC & Hr_adv & Hregs & Hown & Hprog & #Hwadv & #Hmalloc & Hpc_b & Ha_entry & Ha_entry' & Ha_env & #Hflag) Hφ". 
+    iIntros (Hvpc Hcont Hwb1 Hwb2 Ha_entry Ha_entry' Ha_env Hdom φ)
+            "(HPC & Hr_adv & Hregs & Hown & Hprog & #Hwadv & #Hmalloc & Hpc_b & Ha_entry & Ha_entry' & Ha_env & #Hflag) Hφ".
     (* extract r_t0 *)
     assert (is_Some (rmap !! r_t0)) as [w0 Hw0].
     { apply elem_of_gmap_dom. rewrite Hdom. clear;set_solver. }
-    iDestruct (big_sepM_delete with "Hregs") as "[Hr_t0 Hregs]";[apply Hw0|]. 
+    iDestruct (big_sepM_delete with "Hregs") as "[Hr_t0 Hregs]";[apply Hw0|].
     (* put back r_adv *)
-    iDestruct (big_sepM_insert with "[$Hregs $Hr_adv]") as "Hregs". 
+    iDestruct (big_sepM_insert with "[$Hregs $Hr_adv]") as "Hregs".
     { rewrite lookup_delete_ne;auto. apply elem_of_gmap_dom_none. rewrite Hdom. clear;set_solver. }
 
     (* prepare the program addresses for malloc *)
@@ -185,7 +185,7 @@ Section roe.
     { rewrite !dom_insert_L !dom_delete_L Hdom. set_solver by lia. }
     iSplitR;[iNext;auto|].
     iNext. iIntros "(HPC & Hmalloc_prog & Hpc_b & Ha_entry & Hbe & Hr_t0 & Hown & Hregs)".
-    iDestruct "Hbe" as (b e Hincr) "(Hr_t1 & Hbe)". 
+    iDestruct "Hbe" as (b e Hincr) "(Hr_t1 & Hbe)".
     iDestruct (region_mapsto_single with "Hbe") as (cellv) "(Hbe & _)". revert Hincr; clear; solve_addr.
 
     (* extract r_env and r_t7 *)
@@ -200,33 +200,33 @@ Section roe.
     (* continue *)
     iDestruct (big_sepL2_length with "Hprog") as %Hlength_rest.
     destruct ai_rest as [|? ai_rest];[inversion Hlength_rest|].
-    apply contiguous_between_cons_inv_first in Hcont_rest as Heq; subst a. 
+    apply contiguous_between_cons_inv_first in Hcont_rest as Heq; subst a.
     (* move r_env r_t1 *)
     destruct ai_rest as [|? ai_rest];[inversion Hlength_rest|].
     iPrologue "Hprog".
     iApply (wp_move_success_reg with "[$HPC $Hi $Hr_env $Hr_t1]");
-      [apply decode_encode_instrW_inv|iCorrectPC a_malloc_end a_last|iContiguous_next Hcont_rest 0|]. 
+      [apply decode_encode_instrW_inv|iCorrectPC a_malloc_end a_last|iContiguous_next Hcont_rest 0|].
     iEpilogue "(HPC & Hi & Hr_env & Hr_t1)". iCombine "Hi" "Hmalloc_prog" as "Hprog_done".
     (* move r_t7 r_t1 *)
     destruct ai_rest as [|? ai_rest];[inversion Hlength_rest|].
     iPrologue "Hprog".
     iApply (wp_move_success_reg with "[$HPC $Hi $Hr_t7 $Hr_t1]");
-      [apply decode_encode_instrW_inv|iCorrectPC a_malloc_end a_last|iContiguous_next Hcont_rest 1|]. 
-    iEpilogue "(HPC & Hi & Hr_t7 & Hr_t1)". iCombine "Hi" "Hprog_done" as "Hprog_done". 
+      [apply decode_encode_instrW_inv|iCorrectPC a_malloc_end a_last|iContiguous_next Hcont_rest 1|].
+    iEpilogue "(HPC & Hi & Hr_t7 & Hr_t1)". iCombine "Hi" "Hprog_done" as "Hprog_done".
     (* store r_env 1 *)
     destruct ai_rest as [|? ai_rest];[inversion Hlength_rest|].
     iPrologue "Hprog".
     iApply (wp_store_success_z with "[$HPC $Hi $Hr_env $Hbe]");
       [apply decode_encode_instrW_inv|iCorrectPC a_malloc_end a_last|iContiguous_next Hcont_rest 2|..]; auto.
     { rewrite andb_true_iff Z.leb_le Z.ltb_lt. clear -Hincr. solve_addr. }
-    iEpilogue "(HPC & Hi & Hr_env & Hbe)". iCombine "Hi" "Hprog_done" as "Hprog_done". 
+    iEpilogue "(HPC & Hi & Hr_env & Hbe)". iCombine "Hi" "Hprog_done" as "Hprog_done".
     (* restrict r_t7 RO *)
     destruct ai_rest as [|? ai_rest];[inversion Hlength_rest|].
     iPrologue "Hprog".
     iApply (wp_restrict_success_z with "[$HPC $Hi $Hr_t7]");
       [apply decode_encode_instrW_inv|iCorrectPC a_malloc_end a_last|iContiguous_next Hcont_rest 3|auto..].
     { rewrite decode_encode_perm_inv. auto. }
-    iEpilogue "(HPC & Hi & Hr_t7)". iCombine "Hi" "Hprog_done" as "Hprog_done". 
+    iEpilogue "(HPC & Hi & Hr_t7)". iCombine "Hi" "Hprog_done" as "Hprog_done".
 
     (* prepare the program addresses for call *)
     iDestruct (contiguous_between_program_split with "Hprog") as
@@ -245,7 +245,7 @@ Section roe.
     { eapply isCorrectPC_range_restrict. apply Hvpc.
       generalize (contiguous_between_bounds _ _ _ Hcont_call).
       generalize (contiguous_between_bounds _ _ _ Hcont_malloc).
-      apply contiguous_between_middle_bounds' with (ai:=a2) in Hcont_rest;[|repeat constructor]. 
+      apply contiguous_between_middle_bounds' with (ai:=a2) in Hcont_rest;[|repeat constructor].
       clear -Hcont_rest; solve_addr. }
     (* prepare the registers *)
     iDestruct (big_sepM_delete _ _ r_adv with "Hregs") as "[Hr_adv Hregs]";[rewrite !lookup_delete_ne// !lookup_insert_ne//
@@ -256,21 +256,21 @@ Section roe.
     rewrite - !(delete_insert_ne _ r_t1)// 2!(delete_commute _ _ r_t1)// insert_delete.
     (* apply the call spec *)
     iApply (wp_wand _ _ _ (λ v0 : language.val cap_lang, True ∨ ⌜v0 = FailedV⌝)%I with "[-]");[|auto].
-    rewrite -/(call _ _ _ _). 
+    rewrite -/(call _ _ _ _).
     iApply (call_spec r_adv {[r_env:=WCap RWX b e b]} {[r_t7:=WCap (decodePerm ro) b e b]} _
                       _ (delete r_t7 (delete r_t0 rmap))
               with "[- $HPC $Hown $Hmalloc $Hpc_b $Ha_entry $Hr_adv $Hregs]");
-      [apply Hvpc3|apply Hcont_call|auto|apply Ha_entry|..|solve_ndisj|]. 
+      [apply Hvpc3|apply Hcont_call|auto|apply Ha_entry|..|solve_ndisj|].
     { rewrite map_to_list_singleton. auto. }
     { rewrite !dom_singleton_L dom_insert_L !dom_delete_L !dom_insert_L !dom_delete_L Hdom. clear.
       rewrite !union_assoc_L !difference_difference_L !union_assoc_L union_comm_L (union_comm_L {[r_t2; r_t3; r_t4; r_t5]}).
       rewrite difference_union_distr_l_L. set_solver. }
     { rewrite dom_singleton_L !dom_delete_L Hdom. clear. set_solver. }
-    { rewrite !dom_insert_L !dom_delete_L !dom_insert_L dom_delete_L !union_assoc_L Hdom !difference_difference_L. clear. 
+    { rewrite !dom_insert_L !dom_delete_L !dom_insert_L dom_delete_L !union_assoc_L Hdom !difference_difference_L. clear.
       rewrite - !(union_assoc_L {[r_t1]}). apply union_mono_l. apply subseteq_difference_r;[set_solver|].
       apply union_mono_l. apply subseteq_difference_r;[set_solver|]. apply all_registers_subseteq. }
-    rewrite !map_to_list_singleton. iSimpl. rewrite /call. iFrame "Hcall_prog". 
-    iSplitL "Hr_t7". iNext. iApply big_sepM_singleton. iFrame.  
+    rewrite !map_to_list_singleton. iSimpl. rewrite /call. iFrame "Hcall_prog".
+    iSplitL "Hr_t7". iNext. iApply big_sepM_singleton. iFrame.
     iSplitL "Hr_t0". iNext. eauto.
     iSplitL "Hr_env". iNext. iApply big_sepM_singleton. iFrame.
     (* in anticipation of the result of the call macro, we create the callback now *)
@@ -280,19 +280,19 @@ Section roe.
     iDestruct "Hbc" as (b_c e_c b_l e_l a_end Hnext) "(HPC & Hregs & Hr_t7 & Hpc_b & Ha_entry & Hr_adv & Hr_t0 & Hbec & Hbel & Hcall_prog & Hown)".
     (* cleanup *)
     iDestruct (big_sepM_singleton (λ k i, k ↦ᵣ i)%I with "Hr_t7") as "Hr_t7".
-    iCombine "Hcall_prog" "Hprog_done" as "Hprog_done". 
+    iCombine "Hcall_prog" "Hprog_done" as "Hprog_done".
 
     (* we are now ready to call the unknown adversary *)
     (* we first need to prepare the invariants needed *)
-    iMod (na_inv_alloc logrel_nais _ roeN_act with "Hbec") as "#Hbec". 
+    iMod (na_inv_alloc logrel_nais _ roeN_act with "Hbec") as "#Hbec".
     iMod (na_inv_alloc logrel_nais _ roeN_locals with "Hbel") as "#Hbel".
-    iCombine "Ha_entry' Ha_env Hpc_b Ha_entry" as "Hlink". 
-    iMod (na_inv_alloc logrel_nais _ roeN_link with "Hlink") as "#Hlink". 
-    iMod (inv_alloc (logN.@b) _ (roe_inv b) with "[Hbe]") as "#Hb". 
+    iCombine "Ha_entry' Ha_env Hpc_b Ha_entry" as "Hlink".
+    iMod (na_inv_alloc logrel_nais _ roeN_link with "Hlink") as "#Hlink".
+    iMod (inv_alloc (logN.@b) _ (roe_inv b) with "[Hbe]") as "#Hb".
     { iNext. iExists _; iFrame. auto. }
     iMod (na_inv_alloc logrel_nais _ roeN_prog with "Hprog") as "#Hprog".
     iClear "Hprog_done".
-    
+
     (* Let's assert that the continuation holds *)
     iDestruct (big_sepM_to_create_gmap_default _ _ (λ k i, k ↦ᵣ i)%I (WInt 0%Z) with "Hregs")  as "Hregs";[apply Permutation_refl|reflexivity|].
     iDestruct (big_sepM_insert with "[$Hregs $Hr_adv]") as "Hregs".
@@ -305,7 +305,7 @@ Section roe.
     match goal with |- context [ ([∗ map] k↦y ∈ ?regs, k ↦ᵣ y)%I ] =>
           set rmap2 := regs
     end.
-    iSpecialize ("Hcallback_now" $! rmap2). rewrite /interp_expr. 
+    iSpecialize ("Hcallback_now" $! rmap2). rewrite /interp_expr.
 
     iApply (wp_wand with "[-]"). iApply "Hcallback_now". 3: by eauto.
     { iPureIntro. rewrite !dom_insert_L create_gmap_default_dom list_to_set_map_to_list !dom_delete_L Hdom.
@@ -462,5 +462,5 @@ Section roe.
       apply create_gmap_default_lookup_is_Some in Hsome as [Hsome ->]. rewrite !fixpoint_interp1_eq.
       iIntros (?). simplify_eq. done. iIntros (?). done. }
   Qed.
-    
-End roe. 
+
+End roe.
