theories/examples/lse_adequacy.v
@@ -1,0 +1,122 @@
+From iris.algebra Require Import auth agree excl gmap gset frac.
+From iris.proofmode Require Import tactics.
+From iris.base_logic Require Import invariants.
+From iris.program_logic Require Import adequacy.
+From cap_machine Require Import
+     stdpp_extra iris_extra
+     rules logrel fundamental.
+From cap_machine.examples Require Import addr_reg_sample malloc macros_new lse.
+From cap_machine.examples Require Export mkregion_helpers disjoint_regions_tactics.
+From cap_machine.examples Require Import template_adequacy.
+
+Instance DisjointList_list_Addr : DisjointList (list Addr).
+Proof. exact (@disjoint_list_default _ _ app []). Defined.
+
+Import with_adv.
+
+Class memory_layout `{MachineParameters} := {
+  (* Code of f *)
+  f_region_start : Addr;
+  f_start : Addr;
+  f_end : Addr;
+  f_size: (f_start + (length (roe_instrs 0 1 r_adv)) = Some f_end)%a;
+  f_region_start_offset: (f_region_start + 1)%a = Some f_start;
+
+  (* adversary code *)
+  adv_start : Addr;
+  adv_end : Addr;
+  adv_instrs : list Word;
+  adv_size : (adv_start + (length adv_instrs) = Some adv_end)%a ;
+
+  (* malloc routine *)
+  malloc_start : Addr;
+  malloc_memptr : Addr;
+  malloc_mem_start : Addr;
+  malloc_end : Addr;
+
+  malloc_code_size :
+    (malloc_start + length malloc_subroutine_instrs)%a
+    = Some malloc_memptr;
+
+  malloc_memptr_size :
+    (malloc_memptr + 1)%a = Some malloc_mem_start;
+
+  malloc_mem_size :
+    (malloc_mem_start <= malloc_end)%a;
+
+  (* fail routine *)
+  fail_start : Addr;
+  fail_end : Addr;
+
+  fail_size :
+    (fail_start
+     + (length assert_fail_instrs (* code of the subroutine *)
+        + 1 (* pointer to the flag *))
+    )%a
+    = Some fail_end;
+
+  (* link table *)
+  link_table_start : Addr;
+  link_table_end : Addr;
+
+  link_table_size :
+    (link_table_start + 2)%a = Some link_table_end;
+
+  (* failure flag *)
+  fail_flag : Addr;
+  fail_flag_next : Addr;
+  fail_flag_size :
+    (fail_flag + 1)%a = Some fail_flag_next;
+
+  (* disjointness of all the regions above *)
+  regions_disjoint :
+    ## [
+        region_addrs adv_start adv_end;
+        region_addrs f_start f_end;
+        [fail_flag];
+        region_addrs link_table_start link_table_end;
+        region_addrs fail_start fail_end;
+        region_addrs malloc_mem_start malloc_end;
+        [malloc_memptr];
+        region_addrs malloc_start malloc_memptr
+       ]
+}.
+
+Definition mk_initial_memory `{memory_layout} : gmap Addr Word :=
+    mkregion f_start f_end (roe_instrs 0 1 r_adv)
+  ∪ mkregion adv_start adv_end adv_instrs
+  ∪ mkregion 
+
+
+Definition roe_prog `{MachineParameters} `{memory_layout} : prog :=
+  {| prog_start := f_start ;
+     prog_end := f_end ;
+     prog_instrs := (roe_instrs 0 1 r_adv) ;
+     prog_size := f_size |}.
+
+Definition adv_prog `{MachineParameters} `{memory_layout} : prog :=
+  {| prog_start := adv_start ;
+     prog_end := adv_end ;
+     prog_instrs := adv_instrs ;
+     prog_size := adv_size |}.
+
+
+Definition OK_invariant `{MachineParameters} `{memory_layout} (m : gmap Addr Word) : Prop :=
+  ∀ w, m !! fail_flag = Some w → w = WInt 0%Z.
+
+Definition OK_dom `{MachineParameters} `{memory_layout} : gset Addr := {[ fail_flag ]}.
+
+Program Definition OK_dom_correct `{MachineParameters} `{memory_layout} :
+  ∀ m m',
+    (∀ a, a ∈ OK_dom → ∃ x, m !! a = Some x ∧ m' !! a = Some x) →
+    OK_invariant m ↔ OK_invariant m'.
+Proof.
+  intros m m' Hdom.
+  destruct Hdom with fail_flag as [w [Hw1 Hw2] ]. set_solver.
+  split;intros HOK;intros w' Hw';simplify_eq;apply HOK;auto.
+Defined.
+
+Definition flag_inv `{MachineParameters} `{memory_layout} : memory_inv :=
+  {| minv := OK_invariant ;
+     minv_dom := {[ fail_flag ]} ;
+     minv_dom_correct := OK_dom_correct |}.
